src/Resolute_Types.v
@@ -1,5 +1,25 @@
-Require Import Term_Defs Resolute_Logic. (* Attestation_Session AppraisalSummary. *)
+Require Import Term_Defs Resolute_Logic JSON. (* Attestation_Session AppraisalSummary. *)
 (* Require Export Interface_Strings_Vars. *)
+
+Record Resolute_Client_Request := 
+  mkResoluteClientReq {
+    resclientreq_attest_id: string;
+    resclientreq_args: JSON;
+    resclientreq_resultpath: string;
+  }.
+
+Record Resolute_Client_Response := 
+  mkResoluteClientResp {
+    resclientresp_success: bool
+  }.
+
+Record Resolute_Client_Result := 
+  mkResoluteClientResult {
+    resclientres_term: Term;
+    resclientres_evidence: Evidence;
+    resclientres_success: bool;
+    resclientres_error_str: string;
+  }.
 
 
 Record ResoluteResponse := 
